Replace Expr with ArExpr for arithmetic expressions throughout

ExprEval/Basic.lean
@@ -1,46 +1,44 @@
+inductive ArExpr: Type
+    | Const: Int -> ArExpr
+    | Add: ArExpr -> ArExpr -> ArExpr
+    | Sub: ArExpr -> ArExpr -> ArExpr
+    | Mul: ArExpr -> ArExpr -> ArExpr
 
-
-inductive Expr: Type
-    | Const: Int -> Expr
-    | Add: Expr -> Expr -> Expr
-    | Sub: Expr -> Expr -> Expr
-    | Mul: Expr -> Expr -> Expr
-
-def eval (e: Expr): Int :=
+def eval (e: ArExpr): Int :=
     match e with
-        | Expr.Const x => x
-        | Expr.Add lhs rhs => (eval lhs) + (eval rhs)
-        | Expr.Sub lhs rhs => (eval lhs) - (eval rhs)
-        | Expr.Mul lhs rhs => (eval lhs) * (eval rhs)
+        | ArExpr.Const x => x
+        | ArExpr.Add lhs rhs => (eval lhs) + (eval rhs)
+        | ArExpr.Sub lhs rhs => (eval lhs) - (eval rhs)
+        | ArExpr.Mul lhs rhs => (eval lhs) * (eval rhs)
 
 
 -- My small steps semantic
 
-inductive Step: Expr -> Expr -> Prop where
+inductive Step: ArExpr -> ArExpr -> Prop where
     | addConstConst(n1 n2: Int) :
         Step
-            (Expr.Add (Expr.Const n1) (Expr.Const n2))
-            (Expr.Const (n1 + n2))
+            (ArExpr.Add (ArExpr.Const n1) (ArExpr.Const n2))
+            (ArExpr.Const (n1 + n2))
     | subConstConst(n1 n2: Int) :
         Step
-            (Expr.Sub (Expr.Const n1) (Expr.Const n2))
-            (Expr.Const (n1 - n2))
+            (ArExpr.Sub (ArExpr.Const n1) (ArExpr.Const n2))
+            (ArExpr.Const (n1 - n2))
     | mulConstConst(n1 n2: Int) :
         Step
-            (Expr.Mul (Expr.Const n1) (Expr.Const n2))
-            (Expr.Const (n1 * n2))
-    | addLeft (e1 e1' e2) : Step e1 e1' -> Step (Expr.Add e1 e2) (Expr.Add e1' e2)
-    | subLeft (e1 e1' e2) : Step e1 e1' -> Step (Expr.Sub e1 e2) (Expr.Sub e1' e2)
-    | mulLeft (e1 e1' e2) : Step e1 e1' -> Step (Expr.Mul e1 e2) (Expr.Mul e1' e2)
-    | addRight (n: Int) (e2 e2': Expr) : Step e2 e2' -> Step (Expr.Add (Expr.Const n) e2)  (Expr.Add (Expr.Const n) e2')
-    | subRight (n: Int) (e2 e2': Expr) : Step e2 e2' -> Step (Expr.Sub (Expr.Const n) e2)  (Expr.Sub (Expr.Const n) e2')
-    | mulRight (n: Int) (e2 e2': Expr) : Step e2 e2' -> Step (Expr.Mul (Expr.Const n) e2)  (Expr.Mul (Expr.Const n) e2')
+            (ArExpr.Mul (ArExpr.Const n1) (ArExpr.Const n2))
+            (ArExpr.Const (n1 * n2))
+    | addLeft (e1 e1' e2) : Step e1 e1' -> Step (ArExpr.Add e1 e2) (ArExpr.Add e1' e2)
+    | subLeft (e1 e1' e2) : Step e1 e1' -> Step (ArExpr.Sub e1 e2) (ArExpr.Sub e1' e2)
+    | mulLeft (e1 e1' e2) : Step e1 e1' -> Step (ArExpr.Mul e1 e2) (ArExpr.Mul e1' e2)
+    | addRight (n: Int) (e2 e2': ArExpr) : Step e2 e2' -> Step (ArExpr.Add (ArExpr.Const n) e2)  (ArExpr.Add (ArExpr.Const n) e2')
+    | subRight (n: Int) (e2 e2': ArExpr) : Step e2 e2' -> Step (ArExpr.Sub (ArExpr.Const n) e2)  (ArExpr.Sub (ArExpr.Const n) e2')
+    | mulRight (n: Int) (e2 e2': ArExpr) : Step e2 e2' -> Step (ArExpr.Mul (ArExpr.Const n) e2)  (ArExpr.Mul (ArExpr.Const n) e2')
 
-inductive StepStar : Expr → Expr → Prop where
+inductive StepStar : ArExpr → ArExpr → Prop where
     | refl e : StepStar e e
     | trans e₁ e₂ e₃ : Step e₁ e₂ → StepStar e₂ e₃ → StepStar e₁ e₃
 
-theorem step_preserve_eval (e e': Expr): Step e e' -> eval e = eval e' := by
+theorem step_preserve_eval (e e': ArExpr): Step e e' -> eval e = eval e' := by
     intro h
     induction h with
 
@@ -56,17 +54,17 @@ theorem step_preserve_eval (e e': Expr): Step e e' -> eval e = eval e' := by
     | subRight n e2 e1' _ ih
     | mulRight n e2 e1' _ ih => simp [eval, ih]
 
-theorem stepstar_preserves_eval (e e': Expr) : StepStar e e' → eval e = eval e' := by
+theorem stepstar_preserves_eval (e e': ArExpr) : StepStar e e' → eval e = eval e' := by
     intro h
     induction h with
     | refl _ => rfl
     | trans _ _ _ h1 _ ih => rw [step_preserve_eval _ _ h1, ih]
 
-theorem soundness (e: Expr) (v: Int) : StepStar e (Expr.Const v) → eval e = v := by
+theorem soundness (e: ArExpr) (v: Int) : StepStar e (ArExpr.Const v) → eval e = v := by
     exact stepstar_preserves_eval _ _
 
-theorem stepstar_add_left (e1 e1' e2: Expr) :
-    StepStar e1 e1' → StepStar (Expr.Add e1 e2) (Expr.Add e1' e2) := by
+theorem stepstar_add_left (e1 e1' e2: ArExpr) :
+    StepStar e1 e1' → StepStar (ArExpr.Add e1 e2) (ArExpr.Add e1' e2) := by
     intro h
     induction h with
     | refl _ => apply StepStar.refl
@@ -75,8 +73,8 @@ theorem stepstar_add_left (e1 e1' e2: Expr) :
         . exact Step.addLeft _ _ _ step
         . exact ih
 
-theorem stepstar_add_right (n: Int) (e2 e2': Expr) :
-    StepStar e2 e2' → StepStar (Expr.Add (Expr.Const n) e2) (Expr.Add (Expr.Const n) e2') := by
+theorem stepstar_add_right (n: Int) (e2 e2': ArExpr) :
+    StepStar e2 e2' → StepStar (ArExpr.Add (ArExpr.Const n) e2) (ArExpr.Add (ArExpr.Const n) e2') := by
     intro h
     induction h with
     | refl _ => apply StepStar.refl
@@ -87,8 +85,8 @@ theorem stepstar_add_right (n: Int) (e2 e2': Expr) :
 
 
 
-theorem stepstar_sub_left (e1 e1' e2: Expr) :
-    StepStar e1 e1' → StepStar (Expr.Sub e1 e2) (Expr.Sub e1' e2) := by
+theorem stepstar_sub_left (e1 e1' e2: ArExpr) :
+    StepStar e1 e1' → StepStar (ArExpr.Sub e1 e2) (ArExpr.Sub e1' e2) := by
     intro h
     induction h with
     | refl _ => apply StepStar.refl
@@ -97,8 +95,8 @@ theorem stepstar_sub_left (e1 e1' e2: Expr) :
         . exact Step.subLeft _ _ _ step
         . exact ih
 
-theorem stepstar_sub_right (n: Int) (e2 e2': Expr) :
-    StepStar e2 e2' → StepStar (Expr.Sub (Expr.Const n) e2) (Expr.Sub (Expr.Const n) e2') := by
+theorem stepstar_sub_right (n: Int) (e2 e2': ArExpr) :
+    StepStar e2 e2' → StepStar (ArExpr.Sub (ArExpr.Const n) e2) (ArExpr.Sub (ArExpr.Const n) e2') := by
     intro h
     induction h with
     | refl _ => apply StepStar.refl
@@ -109,8 +107,8 @@ theorem stepstar_sub_right (n: Int) (e2 e2': Expr) :
 
 
 
-theorem stepstar_mul_left (e1 e1' e2: Expr) :
-    StepStar e1 e1' → StepStar (Expr.Mul e1 e2) (Expr.Mul e1' e2) := by
+theorem stepstar_mul_left (e1 e1' e2: ArExpr) :
+    StepStar e1 e1' → StepStar (ArExpr.Mul e1 e2) (ArExpr.Mul e1' e2) := by
     intro h
     induction h with
     | refl _ => apply StepStar.refl
@@ -119,8 +117,8 @@ theorem stepstar_mul_left (e1 e1' e2: Expr) :
         . exact Step.mulLeft _ _ _ step
         . exact ih
 
-theorem stepstar_mul_right (n: Int) (e2 e2': Expr) :
-    StepStar e2 e2' → StepStar (Expr.Mul (Expr.Const n) e2) (Expr.Mul (Expr.Const n) e2') := by
+theorem stepstar_mul_right (n: Int) (e2 e2': ArExpr) :
+    StepStar e2 e2' → StepStar (ArExpr.Mul (ArExpr.Const n) e2) (ArExpr.Mul (ArExpr.Const n) e2') := by
     intro h
     induction h with
     | refl _ => apply StepStar.refl
@@ -129,7 +127,7 @@ theorem stepstar_mul_right (n: Int) (e2 e2': Expr) :
         . apply Step.mulRight _ _ _ step1
         . exact ih
 
-theorem chasle_step_star {e1 e2 e3: Expr}: StepStar e1 e2 -> StepStar e2 e3 -> StepStar e1 e3 := by
+theorem chasle_step_star {e1 e2 e3: ArExpr}: StepStar e1 e2 -> StepStar e2 e3 -> StepStar e1 e3 := by
     intros h1 h2
     induction h1 with
     | refl e => exact h2
@@ -138,38 +136,38 @@ theorem chasle_step_star {e1 e2 e3: Expr}: StepStar e1 e2 -> StepStar e2 e3 -> S
         have h4 := StepStar.trans _ _ _ step h3
         exact h4
 
-theorem completeness (e: Expr) : StepStar e (Expr.Const (eval e)) := by
+theorem completeness (e: ArExpr) : StepStar e (ArExpr.Const (eval e)) := by
     induction e with
     | Const x =>
         simp [eval]
         exact StepStar.refl _
     | Add e1 e2 ih1 ih2 =>
-        -- ih1 : StepStar e1 (Expr.Const (eval e1))
-        -- ih2 : StepStar e2 (Expr.Const (eval e2))
+        -- ih1 : StepStar e1 (ArExpr.Const (eval e1))
+        -- ih2 : StepStar e2 (ArExpr.Const (eval e2))
         simp [eval]
         have a := stepstar_add_left _ _ e2 ih1
         have b := stepstar_add_right (eval e1) e2 _ ih2
         have c := Step.addConstConst (eval e1) (eval e2)
-        have d := StepStar.trans _ _ _ c (StepStar.refl (Expr.Const (eval e1 + eval e2)))
+        have d := StepStar.trans _ _ _ c (StepStar.refl (ArExpr.Const (eval e1 + eval e2)))
         have e := chasle_step_star a (chasle_step_star b d)
         exact e
     | Sub e1 e2 ih1 ih2 =>
-        -- ih1 : StepStar e1 (Expr.Const (eval e1))
-        -- ih2 : StepStar e2 (Expr.Const (eval e2))
+        -- ih1 : StepStar e1 (ArExpr.Const (eval e1))
+        -- ih2 : StepStar e2 (ArExpr.Const (eval e2))
         simp [eval]
         have a := stepstar_sub_left _ _ e2 ih1
         have b := stepstar_sub_right (eval e1) e2 _ ih2
         have c := Step.subConstConst (eval e1) (eval e2)
-        have d := StepStar.trans _ _ _ c (StepStar.refl (Expr.Const (eval e1 - eval e2)))
+        have d := StepStar.trans _ _ _ c (StepStar.refl (ArExpr.Const (eval e1 - eval e2)))
         have e := chasle_step_star a (chasle_step_star b d)
         exact e
     | Mul e1 e2 ih1 ih2 =>
-        -- ih1 : StepStar e1 (Expr.Const (eval e1))
-        -- ih2 : StepStar e2 (Expr.Const (eval e2))
+        -- ih1 : StepStar e1 (ArExpr.Const (eval e1))
+        -- ih2 : StepStar e2 (ArExpr.Const (eval e2))
         simp [eval]
         have a := stepstar_mul_left _ _ e2 ih1
         have b := stepstar_mul_right (eval e1) e2 _ ih2
         have c := Step.mulConstConst (eval e1) (eval e2)
-        have d := StepStar.trans _ _ _ c (StepStar.refl (Expr.Const (eval e1 * eval e2)))
+        have d := StepStar.trans _ _ _ c (StepStar.refl (ArExpr.Const (eval e1 * eval e2)))
         have e := chasle_step_star a (chasle_step_star b d)
         exact e
